\documentclass[a4paper,12pt]{report}

\usepackage{../courslatex}
\usepackage{exos}
\usepackage{enumitem}

\setlist[enumerate]{align=left,leftmargin=1cm,itemsep=5pt,parsep=0pt,topsep=0pt,rightmargin=0.5cm}

\setlist[itemize]{align=left,labelsep=1em,leftmargin=*,itemsep=0pt,parsep=0pt,topsep=0pt,rightmargin=0cm}

\renewcommand{\titreChapitre}{Ch3 : Calcul littéral} 
\renewcommand{\numeroSerie}{5}

\begin{document}
\vspace*{-2\baselineskip}
\textLigne{Exercices}
\begin{core}
c.f. théorie C3
\end{core}
\begin{core}
Un nombre pair $a$ s'écrit $a=2n$ pour $n\in \N$, un nombre impair $b$ s'écrit $b=2m+1$ pour $m\in \N$. On a 
\[a+b=2n+2m+1=2(n+m)+1=2k+1 \text{ avec } k=n+m\]
et donc $a+b$ est bien un nombre impair.
\end{core}
\begin{core}
	\phantom{ }
	\begin{tasks}(4)
\task $x^2 + 2xy + y^2$
\task $4x^4 - 4x^2 - 12$
\task $x^2 - y^2$
\task $9x^2 + 6xy + y^2$
\task $x^4 + 2x^2y^3 + y^6$
\task $x^2 - 2x + 1$
\task $1 - x^2$
\task $16x^2 - 24x + 9$
\task $x^6 - 9y^2$
\task $9z^2 - 12z + 4$
\task $x^2 - 2x +1$
\task $x^2y^2 + 4xy^2 + 4y^2$
\task $x^4 - 2x^2 + 1$
\task $4x^2 + 8x + 4$
\task $4a^2 + 12a + 9$
\task $x^2y^2z^2 - 25$
\task $9x^6 - 30x^3 + 25$
\task $a^2 + 6ab + 9b^2$
\task $x^4 - 2x^2 + 1$
\task $16a^4b^2 - 25$
\task $4x^2y^6 - 4xy^3 + 1$
\task $x^8 + 2x^4y + y^2$
\task $1 - a^2x^8$
\task $x^4 - a^4$
	\end{tasks}
\end{core}

\begin{core}
	\phantom{ }
	\begin{tasks}(4)
\task $ x^2 - 3x + 2$
\task $ x^2 + 4x + 3$
\task $ x^2 - 16$
\task $ y^2 - 2y - 48$
\task $ a^2 - 11a - 12$
\task $ y^2 + 5y - 36$
\task $ a^2 + 10a + 21$
\task $ x^2 - 13x + 30$
\end{tasks}
\end{core}

\begin{core}
	Par exemple, $23^2=(20+3)^2=20^2+2\cdot 20\cdot 3+3^9=400+120+9=529$.
\end{core}
\begin{core}
	\phantom{ }
	\begin{tasks}(2)
\task $a + b$
\task $a^2 + 2ab + b^2$
\task $a^3 + 3a^2b + 3ab^2 + b^3$
\task $a^4 + 4a^3b + 6a^2b^2 + 4ab^3 + b^4$
\task $a^5 + 5a^4b + 10a^3b^2 + 10a^2b^3 + 5ab^4 + b^5$
	\end{tasks}
\end{core}
\begin{core}\phantom{ }

\begin{tasks}(3)
\task $100 r^2 x^2 + 130 r x + 40 $
\task $s^2 t^2-\dfrac{9}{4} s^2$
\task $25 s^4 y^2-\dfrac{25}{4} s^4 y + \dfrac{25}{64} s^4$
\task $\dfrac{4}{9} s^2 x^2 + \dfrac{1}{6} s x^2 + \dfrac{1}{64} x^2$
\task $-\dfrac{9}{25} r^4 z^2 + \dfrac{4}{25} z^4$
\task $16 r^2 t^4-28 r^2 t^2 + \dfrac{49}{4} r^2$
\task $36 r^2 y^2 + 30 r y + 6 $
\task $\dfrac{16}{9} z^4 + \dfrac{40}{27} r z^3 + \dfrac{25}{81} r^2 z^2$
\task $\dfrac{16}{49} t^2 x^2-\dfrac{4}{7} t x-56 $
\task $\dfrac{64}{49} t^6 + \dfrac{160}{7} s t^3 + 100 s^2$
\end{tasks}

\end{core}


\textLigne{Automatismes}


\begin{core}\phantom{ }

\begin{tasks}(2)
\task $\left(-3 \sqrt{3} +5\sqrt{5}\right)^{2}=
                    \left(-3 \sqrt{3} \right)^{2}+2\cdot (-3)\sqrt{3}\cdot 5\sqrt{5}+\left(5\sqrt{5}\right)^{2}$\\
                    $\phantom{\left(-3 \sqrt{3} +5\sqrt{5}\right)^{2}}=(-3)^{2}\cdot 3 +2\cdot (-3)
                    \cdot \sqrt{3}\cdot 5    \cdot\sqrt{5}+ 25\cdot 5$\\
                    $\phantom{\left(-3 \sqrt{3} +5\sqrt{5}\right)^{2}}=27 -30\sqrt{3\cdot5} +125$\\$\phantom{\left(-3 \sqrt{3} +5\sqrt{5}\right)^{2}}={{152-30\sqrt{15}}}$
\task $\left(6 \sqrt{3} +6\right)\left(6 \sqrt{3}-6\right)=\left(6 \sqrt{3} \right)^{2}-6^{2}$\\
                    $\phantom{\left(6 \sqrt{3} +6\right)\left(6 \sqrt{3}-6\right)}=6^{2}\cdot 3-36$\\
                        $\phantom{\left(6 \sqrt{3} +6\right)\left(6 \sqrt{3}-6\right)}=108-36$\\$\phantom{\left(6 \sqrt{3} +6\right)\left(6 \sqrt{3}-6\right)}={{72}}$
\task $\left(-3 \sqrt{2} +5\sqrt{2}\right)\left(-3 \sqrt{2}-5\sqrt{2}\right)=\left(-3 \sqrt{2} \right)^{2}-\left(5\sqrt{2}\right)^{2}$\\
                $\phantom{\left(-3 \sqrt{2} +5\sqrt{2}\right)\left(-3 \sqrt{2}-5\sqrt{2}\right)}=(-3)^{2}\cdot 2-5^{2}\cdot 2$\\
                    $\phantom{\left(-3 \sqrt{2} +5\sqrt{2}\right)\left(-3 \sqrt{2}-5\sqrt{2}\right)}=18-50$\\$\phantom{\left(-3 \sqrt{2} +5\sqrt{2}\right)\left(-3 \sqrt{2}-5\sqrt{2}\right)}={{-32}}$
\task $\left(-5 \sqrt{2} +5\right)^{2}=\left(-5 \sqrt{2} \right)^{2}+2\cdot (-5)\sqrt{2}\cdot 5+5^{2}$\\
                    $\phantom{\left(-5 \sqrt{2} +5\right)^{2}}=(-5)^{2}\cdot 2 -50\sqrt{2}+ 25$\\
                    $\phantom{\left(-5 \sqrt{2} +5\right)^{2}}=50-50\sqrt{2}+25$\\$\phantom{\left(-5 \sqrt{2} +5\right)^{2}}={{75-50\sqrt{2}}}$
\task $\left(4 \sqrt{3} -6\right)^{2}=\left(4 \sqrt{3} \right)^{2}-2\cdot 4\sqrt{3}\cdot 6+6^{2}$\\
                    $\phantom{\left(4 \sqrt{3} -6\right)^{2}}=4^{2}\cdot 3 -48\sqrt{3}+ 36$\\
                    $\phantom{\left(4 \sqrt{3} -6\right)^{2}}=48-48\sqrt{3}+36$\\$\phantom{\left(4 \sqrt{3} -6\right)^{2}}={{84-48\sqrt{3}}}$
\task $\left(-2 \sqrt{11} -5\right)^{2}=\left(-2 \sqrt{11} \right)^{2}-2\cdot (-2)\sqrt{11}\cdot 5+5^{2}$\\
                    $\phantom{\left(-2 \sqrt{11} -5\right)^{2}}=(-2)^{2}\cdot 11 +20\sqrt{11}+ 25$\\
                    $\phantom{\left(-2 \sqrt{11} -5\right)^{2}}=44+20\sqrt{11}+25$\\$\phantom{\left(-2 \sqrt{11} -5\right)^{2}}={{69+20\sqrt{11}}}$
\end{tasks}

\end{core}

\begin{core}\phantom{ }

\begin{tasks}(2)
\task $5 (8 t y-2 t^2 + 7 y)$ ou $-5 (-8 t y + 2 t^2-7 y)$
\task $4 s(3 s t + 8 s + 6 t)$
\task $5 (-6 z + 9 t + 2 )$ ou $-5 (6 z-9 t-2 )$
\task $10 z(7 s z + 5 s + 6 )$
\task $10 r(5 s^2 + 4 r + 2 )$
\task $7 (3 t + 8 )$
\task $8 x(9 r x + 4 x-7 )$ ou $-8 x(-9 r x-4 x + 7 )$
\task $-7 y(9 y + 8 x + 6 )$
\task $8 (-7 s y-5 s + 3 )$ ou $-8 (7 s y + 5 s-3 )$
\task $3 t(-2 s^2 + 3 t^2)$ ou $-3 t(2 s^2-3 t^2)$
\end{tasks}

\end{core}

\begin{core}\phantom{ }

\begin{tasks}
\task $-6 z(10 r s y + 8 s + 3 )$
\task $10 r t x(-3 r t x-6 r t + x)$ ou $-10 r t x(3 r t x + 6 r t-x)$
\task $7 s(-3 t x z + 6 x z + 8 )$ ou $-7 s(3 t x z-6 x z-8 )$
\task $2 s(-y z^2-8 t + 7 )$ ou $-2 s(y z^2 + 8 t-7 )$
\task $2 s t x(5 t x y-7 s)$ ou $-2 s t x(-5 t x y + 7 s)$
\task $3 z(-6 r x z + 7 t-5 )$ ou $-3 z(6 r x z-7 t + 5 )$
\task $r t(s + 7 )$
\task $8 r t x(7 y^2 + 6 x)$
\task $7 x(5 r x^2 + 6 y z^2)$
\task $3 (-r y + 5 y + 5 )$ ou $-3 (r y-5 y-5 )$
\end{tasks}

\end{core}




\end{document}

