\documentclass[a4paper,12pt]{report}

\usepackage{../courslatex}
\usepackage{exos}
\usepackage{enumitem}

\setlist[enumerate]{align=left,leftmargin=1cm,itemsep=5pt,parsep=0pt,topsep=0pt,rightmargin=0.5cm}

\setlist[itemize]{align=left,labelsep=1em,leftmargin=*,itemsep=0pt,parsep=0pt,topsep=0pt,rightmargin=0cm}

\renewcommand{\titreChapitre}{Ch3 : Des Nombres} 
\renewcommand{\typeDoc}{Corrigé série }
\renewcommand{\numeroSerie}{6}

\begin{document}
\vspace*{-2\baselineskip}
\textLigne{Exercices}

\begin{core}\phantom{ }

\begin{tasks}(2)
\task $9 s^2 z^2-20 s z^2 + {{\dfrac{100}{9} z^2}}={{\left(3 s z-\dfrac{10}{3} z\right)^2}}$
\task $-\dfrac{2}{3} r z + \dfrac{1}{9}  + {{r^2 z^2}}={{\left(r z-\dfrac{1}{3} \right)^2}}$
\task $-\dfrac{49}{9}  + {{s^4}}={{\left(s^2- \dfrac{7}{3} \right)\left(s^2+\dfrac{7}{3} \right)}}$
\task $\dfrac{9}{64} r^2 t^2 + \dfrac{3}{20} r t x + {{\dfrac{1}{25} x^2}}={{\left(\dfrac{3}{8} r t+\dfrac{1}{5} x\right)^2}}$
\task $14 r z + 49  + {{r^2 z^2}}={{\left(r z+7 \right)^2}}$
\task $36 x^2 y^2- {{25 s^2 y^2}}={{\left(6 x y+ 5 s y\right)\left(6 x y-5 s y\right)}}$
\task $\dfrac{25}{9} x^2 + 64 r^4- {{\dfrac{80}{3} r^2 x}}={{\left(8 r^2-\dfrac{5}{3} x\right)^2}}$
\task $s^2 y^2 + 6 s y + {{9 }}={{\left(s y+3 \right)^2}}$
\task $\dfrac{16}{25} -\dfrac{8}{5} x z + {{x^2 z^2}}={{\left(x z-\dfrac{4}{5} \right)^2}}$
\task $16 r^4 + \dfrac{40}{3} r^2 z + {{\dfrac{25}{9} z^2}}={{\left(\dfrac{5}{3} z+4 r^2\right)^2}}$
\end{tasks}

\end{core}

\begin{core}
	\phantom{}
	\begin{tasks}(2)
		\task $(m+n)(a-b)$
		\task $(x-y)(2a-b)$
		\task $(a+1)(x-y)$
		\task $(-2a+b)(x-3y)$
		\task*(2) $(a+b-1)(a+b)^2$
		\task*(2) $(x-3)(x+1)-(x-3)+2(x-3)^2=(x-3)(3x-6)=3(x-3)(x-2)$
		\task*(2) $(a-b)((a-b)^2-1)=(a-b)(a-b+1)(a-b-1)$
		\task*(2) $(x-y)(1-(a+b)^2)=(x-y)(1-a-b)(1+a+b)$
	\end{tasks}
\end{core}

\textLigne{Automatismes}

\begin{core}\phantom{ }

\begin{tasks}
\task ${{10 z(3 s^2 t + s-3 )}}$ ou ${{-10 z(-3 s^2 t-s + 3 )}}$
\task ${{6 t^2 z(9 r t z-r t-3 )}}$ ou ${{-6 t^2 z(-9 r t z + r t + 3 )}}$
\task ${{9 x(-5 r^2 t-3 r + 8 )}}$ ou ${{-9 x(5 r^2 t + 3 r-8 )}}$
\task ${{5 s y(8 s y^2 + 5 s x^2 + 9 x)}}$
\task ${{-10 s x^2(2 x^2 + 2 z + 9 s)}}$
\task ${{2 y z^2(5 y^2 + 10 z^2-3 )}}$ ou ${{-2 y z^2(-5 y^2-10 z^2 + 3 )}}$
\end{tasks}

\end{core}

\begin{core}\phantom{ }

\begin{tasks}(3)
\task ${{\left(6 t-x\right)^2}}$
\task ${{\left(7 r s- 5 \right)\left(7 r s+5 \right)}}$
\task ${{\left(4 x z+5 \right)^2}}$
\task ${{\left(4 r s+7 \right)^2}}$
\task ${{\left(2 z^2-3 \right)^2}}$
\task ${{\left(2 x-7 s^2\right)^2}}$
\task ${{\left(6 r+ 5 t^2\right)\left(6 r-5 t^2\right)}}$
\task ${{\left(r y-7 \right)^2}}$
\task ${{\left(6 r t- 7 \right)\left(6 r t+7 \right)}}$
\task ${{\left(8 x+7 \right)^2}}$
\end{tasks}

\end{core}

\begin{core}\phantom{ }

\begin{tasks}(3)
\task ${{\left(4 t-7 y z^2\right)^2}}$
\task ${{\left(2 x^2-7 s\right)^2}}$
\task ${{\left(6 r s x+7 \right)^2}}$
\task ${{\left(10 r-7 y\right)^2}}$
\task ${{\left(4 s y z-3 \right)^2}}$
\task ${{\left(2 x y-z\right)^2}}$
\task ${{\left(7 s-10 r\right)^2}}$
\task ${{\left(2 x-3 \right)^2}}$
\task ${{\left(9 x+4 s^2 y\right)^2}}$
\task ${{\left(5 r x-3 \right)^2}}$
\end{tasks}

\end{core}

\begin{core}\phantom{ }

\begin{tasks}
\task ${{3 r}}\mathopen{}\left(25 r^4 s^2 t^2 + 20 r^2 s t y + 4 y^2\right)\mathclose{}={{3 r\mathopen{}\left(2 y+5 r^2 s t\right)\mathclose{}^2}}$
\task ${{-x}}\mathopen{}\left(25 s^2 t^2 x^2 y^2 + 80 s t x y + 64 \right)\mathclose{}={{-x\mathopen{}\left(5 s t x y+8 \right)\mathclose{}^2}}$
\task ${{-3 r z}}\mathopen{}\left(9 y^2 z^2 + 60 y z + 100 \right)\mathclose{}={{-3 r z\mathopen{}\left(3 y z+10 \right)\mathclose{}^2}}$
\task ${{-2 s^2 z}}\mathopen{}\left(64 t^4 x^2-16 s^2 t^2 x z + s^4 z^2\right)\mathclose{}={{-2 s^2 z\mathopen{}\left(8 t^2 x-s^2 z\right)\mathclose{}^2}}$
\task ${{-3 x^2 y}}\mathopen{}\left(9 s^2 y^4 z^2 + 48 s y^2 z + 64 \right)\mathclose{}={{-3 x^2 y\mathopen{}\left(3 s y^2 z+8 \right)\mathclose{}^2}}$
\task ${{3 t x}}\mathopen{}\left(4 t^2 x^2 z^2-12 t x z + 9 \right)\mathclose{}={{3 t x\mathopen{}\left(2 t x z-3 \right)\mathclose{}^2}}$
\task ${{-5 z}}\mathopen{}\left(y^2-16 y + 64 \right)\mathclose{}={{-5 z\mathopen{}\left(y-8 \right)\mathclose{}^2}}$
\task ${{-z}}\mathopen{}\left(r^2 t^2 + 4 r t x^2 + 4 x^4\right)\mathclose{}={{-z\mathopen{}\left(r t+2 x^2\right)\mathclose{}^2}}$
\task ${{-2 t}}\mathopen{}\left(-49 r^2 s^4 + 36 t^2\right)\mathclose{}={{-2 t\mathopen{}\left(6 t+ 7 r s^2\right)\mathclose{}\mathopen{}\left(6 t-7 r s^2\right)\mathclose{}}}$
\task ${{5 r z}}\mathopen{}\left(81 x^2 y^4 z^2-72 r x y^2 z + 16 r^2\right)\mathclose{}={{5 r z\mathopen{}\left(9 x y^2 z-4 r\right)\mathclose{}^2}}$
\end{tasks}

\end{core}

\begin{core}\phantom{ }

\begin{tasks}
\task ${{3 s z^2}}\mathopen{}\left(49  + 112 s z + 64 s^2 z^2\right)\mathclose{}={{3 s z^2\mathopen{}\left(8 s z+7 \right)\mathclose{}^2}}$
\task ${{-2 x}}\mathopen{}\left(36 s^2 x^4 + 49 y^2 + 84 s x^2 y\right)\mathclose{}={{-2 x\mathopen{}\left(6 s x^2+7 y\right)\mathclose{}^2}}$
\task ${{-5 s}}\mathopen{}\left(-72 s z + 81 z^2 + 16 s^2\right)\mathclose{}={{-5 s\mathopen{}\left(9 z-4 s\right)\mathclose{}^2}}$
\task ${{2 s x}}\mathopen{}\left(9 s^2 t^2 + 1-6 s t\right)\mathclose{}={{2 s x\mathopen{}\left(3 s t-1\right)\mathclose{}^2}}$
\task ${{-2 s x}}\mathopen{}\left(-28 s x y + 49 x^2 y^2 + 4 s^2\right)\mathclose{}={{-2 s x\mathopen{}\left(7 x y-2 s\right)\mathclose{}^2}}$
\task ${{5 t}}\mathopen{}\left(60 s t + 25  + 36 s^2 t^2\right)\mathclose{}={{5 t\mathopen{}\left(6 s t+5 \right)\mathclose{}^2}}$
\task ${{2 z}}\mathopen{}\left(-16 s y z + 64 y^2 z^2 + s^2\right)\mathclose{}={{2 z\mathopen{}\left(8 y z-s\right)\mathclose{}^2}}$
\task ${{-3 t z^2}}\mathopen{}\left(49 r^4-140 r^2 t + 100 t^2\right)\mathclose{}={{-3 t z^2\mathopen{}\left(10 t-7 r^2\right)\mathclose{}^2}}$
\task ${{2 z}}\mathopen{}\left(81 z^2 + 100  + 180 z\right)\mathclose{}={{2 z\mathopen{}\left(9 z+10 \right)\mathclose{}^2}}$
\task ${{-3 s x z}}\mathopen{}\left(36 x^2 + s^2 z^2 + 12 s x z\right)\mathclose{}={{-3 s x z\mathopen{}\left(6 x+s z\right)\mathclose{}^2}}$
\end{tasks}

\end{core} \end{document}

